    
\begin{description}
    \item{\textbf{问题}}:\\
Given a string s1, we may represent it as a binary tree by partitioning it to two non-empty substrings recursively.\\
Below is one possible representation of s1 = "great":\\
\\
    great\\
   /     $\backslash$ \\
  gr    eat \\
 /  $\backslash$    /   $\backslash$ \\
g   r  e   at \\
           /  $\backslash$ \\
          a   t \\
To scramble the string, we may choose any non-leaf node and swap its two children. \\
\\
For example, if we choose the node "gr" and swap its two children, it produces a scrambled string "rgeat".\\
\\
    rgeat \\
   /     $\backslash$ \\
  rg    eat \\
 /  $\backslash$    /   $\backslash$ \\
r   g  e   at \\
           /  $\backslash$ \\
          a   t \\
We say that "rgeat" is a scrambled string of "great".\\
\\
Similarly, if we continue to swap the children of nodes "eat" and "at", it produces a scrambled string "rgtae".\\
\\
    rgtae\\
   /     $\backslash$ \\
  rg    tae \\
 /  $\backslash$    /   $\backslash$ \\
r   g  ta  e \\
       /  $\backslash$ \\
      t   a \\
We say that "rgtae" is a scrambled string of "great". \\
\\
Given two strings s1 and s2 of the same length, determine if s2 is a scrambled string of s1.\textit{(leetcode 87)}
    \item{\textbf{DP}} : \fbox{时间复杂度O($n^4$) , 空间复杂度O($n^3$)}
	\\我们假设dp[i][j][l]表示$s1_i, ... s1_{i+l-1}$和$s2_j, ... s2_{j+l-1}$是否互为可转置的.\\
	\\dp的递推关系式:
$$
dp[i][j][l] =
\begin{cases} 
s1[i] == s2[j] & l = 1 \\
\prod_{k=1}^{l-1}(dp[i][j][k] \And dp[i+k][j+k][l-k])||(dp[i][j+l-k][k] \And dp[i+k][j][l-k]) & other
\end{cases}
$$
其中上面的求积符号代表或运算
    \begin{lstlisting}
bool isScramble(string s1, string s2) {
	int n = s1.size();
	if(n == 0 || s1.size() != s2.size() ) return false;
	vector<vector<vector<bool> > > dp(n, vector<vector<bool> >(n, vector<bool>(n+1, false)));
	for(int i = 0; i < n; i++)
		for(int j = 0; j < n; j++)
			dp[i][j][1] = s1[i] == s2[j];
	for(int l = 2; l < n+1; l++){
		for(int i = 0; i <= n - l; i++)
			for(int j = 0; j <= n - l; j++){
				for(int k = 1; k < l; k++){
					dp[i][j][l] = dp[i][j][l] 
								|| (dp[i][j][k] && dp[i+k][j+k][l-k])
								|| (dp[i][j+l-k][k] && dp[i+k][j][l-k]);
				}
			}
	}
	return dp[0][0][n];
}
    \end{lstlisting}
	\textit{这道题困难之处在于敢不敢这么简单粗暴的递推}
\end{description}

